

### 1.3.2. DIFFERENTIAL EQUATIONS WITH VARIABLE COEFFICIENTS

Consider an equation of the form

$$a_0(t)x^{(n)}(t) + a_1(t)x^{(n-1)}(t) + \dots + a_n(t)x(t) = f(t), \quad (1.12)$$

where  $a_i(t)$ ,  $i = 0, 1, \dots, n$  - polynomials of degree  $m_i$ , function  $f(t)$  is the original.

Let's denote  $m = \max \{m_0, m_1, \dots, m_n\}$ .

We will assume that the Cauchy problem for equation (1.12) with the conditions

$$x(0) = x_0, \quad x'(0) = x_1, \quad \dots, \quad x^{(n-1)}(0) = x_{n-1}$$

has a solution on the set of originals.

Let  $x(t) \leftrightarrow X(p)$ .

According to the image differentiation rule, we have

$$t^k x^{(s)}(t) \leftrightarrow (-1)^k \frac{d^k}{dp^k} (L\{x^{(s)}(t)\}) = (-1)^k \frac{d^k}{dp^k} (p^s X(p) - p^{s-1}x_0 - \dots - x_{s-1}).$$

Thus, applying the Laplace transform to both parts of equation (1.12), equation (1.12) is transformed into an  $m$ -th order differential equation with respect to the image  $X(p)$ . After that, the task of integrating equation (1.12) is simplified.

### Example 1

Find a solution to the equation

$$ty''(t) - (1+t)y'(t) + y(t) = 0$$

Solution:

$$y(t) \leftrightarrow Y(p)$$

$$y'(t) \leftrightarrow pY(p) - y(0)$$

Using the image differentiation property ( $tf(t) \leftrightarrow -F'(p)$ ), we have

$$ty'(t) \leftrightarrow -(pY(p) - y(0))' = -(Y(p) + pY'(p)) = -p \frac{dY(p)}{dp} - Y(p),$$

(because  $y(0) = \text{const}$ ).

$$y''(t) \leftrightarrow p^2Y(p) - py(0) - y'(0)$$

$$ty''(t) \leftrightarrow -(p^2Y(p) - py(0) - y'(0))' = -(2pY(p) + p^2Y'(p) - y(0))$$

We substitute the images for these terms into the equation and multiply each term by (-1) to get rid of the numerous minus signs.

We have

$$ty''(t) - y'(t) - ty'(t) + y(t) = 0$$

we substitute and get

$$2pY(p) + p^2Y'(p) - y(0) - (-pY(p) + y(0)) - (Y(p) + pY'(p)) - Y(p) = 0$$

$$2pY(p) + p^2Y'(p) - y(0) + pY(p) - y(0) - Y(p) - pY'(p) - Y(p) = 0$$

$$(p^2 - p)Y'(p) + (3p - 2)Y(p) = 2y(0) = 2C_0$$

let's denote an unknown quantity by  $C_0 = \text{const}$ .

In the image space, we did not get an algebraic equation, as before, we get a first-order differential equation (linear inhomogeneous). First, we solve the corresponding homogeneous equation, when in the right part, instead of the term  $2C_0$ , there is zero.

$$(p^2 - p)Y'(p) + (3p - 2)Y(p) = 0$$

The resulting equation is an equation with separable variables.

Since  $Y'(p) = \frac{dY}{dp}$  then

$$(p^2 - p) \frac{dY}{dp} = -(3p - 2)Y(p)$$

$$\frac{dY}{Y} = -\frac{(3p - 2)}{(p^2 - p)} dp$$

We can integrate and get:

$$\begin{aligned} \ln Y(p) &= -\int \frac{(3p - 2)}{p^2 - p} dp = -\int \frac{(2p - 1)}{p^2 - p} dp - \int \frac{(p - 1)}{p^2 - p} dp = \\ &= -\int \frac{d(p^2 - p)}{(p^2 - p)} - \int \frac{dp}{p} = -\ln(p^2 - p) - \ln p = -\ln(p^3 - p^2) + \ln C \end{aligned}$$

We have received

$$Y_0(p) = \frac{C}{p^3 - p^2}$$

We have set the index to zero, since this is not a solution to our equation.

We use the method of variation of parameters (variation of constants), the Lagrange method to

$$(p^2 - p)Y'(p) + (3p - 2)Y(p) = 2y(0) = 2C_0$$

The solution of an inhomogeneous equation is sought in the same form as the solution of a homogeneous one, only instead of an arbitrary constant  $C$ , a new unknown function  $C(p)$  is put.

$$Y_0(p) = \frac{C}{p^3 - p^2} \rightarrow Y(p) = \frac{C(p)}{p^3 - p^2}$$

This change of variables is substituted into the inhomogeneous equation.

Only first you need to calculate  $Y'(p)$ :

$$Y'(p) = \frac{C'(p)}{p^3 - p^2} - \frac{C(p)(3p^2 - 2p)}{(p^3 - p^2)^2}$$

$$(p^2 - p) \left[ \frac{C'(p)}{p^3 - p^2} - \frac{C(p)(3p^2 - 2p)}{(p^3 - p^2)^2} \right] + (3p - 2) \left[ C(p) \frac{1}{p^3 - p^2} \right] = 2C_0$$

$$\frac{C'(p)}{p} - \frac{C(p)(3p^2 - 2p)}{p(p^3 - p^2)} + \frac{(3p - 2)C(p)}{p^3 - p^2} = 2C_0$$

$$C'(p) = 2C_0 p$$

$$C(p) = C_0 p^2 + C_1$$

Substituting the found function in  $Y(p) = \frac{C(p)}{p^3 - p^2}$  and get

$$Y(p) = \frac{C_0 p^2 + C_1}{p^3 - p^2} = \frac{C_0}{p-1} + \frac{C_1}{(p-1)p^2}$$

From the image of the solution, you need to calculate the inverse Laplace transform (find the original)

$$\frac{1}{p-1} \leftrightarrow e^t$$

For the second term, let's use the property  $(\int_0^t f(u) du \leftrightarrow \frac{F(p)}{p})$ :

$$\frac{1}{p(p-1)} \leftrightarrow \int_0^t e^u du = e^t - 1$$

$$\frac{1}{p^2(p-1)} \leftrightarrow \int_0^t (e^u - 1) du = e^t - 1 - t$$

Our solution is

$$y(t) = C_0 e^t + C_1 (e^t - 1 - t)$$

Let's denote

$$C_0 + C_1 = \tilde{C}_0$$

$$-C_1 = \tilde{C}_1$$

$$y(t) = e^t (C_0 + C_1) + C_1 (-1 - t)$$

$$y(t) = \tilde{C}_0 e^t + \tilde{C}_1 (1 + t)$$

## Example 2

Find a solution to the equation

$$tx''(t) - (1+t)x'(t) + 2(1-t)x(t) = 0.$$

Solution:

Let  $x(t) \leftrightarrow X(p)$ .

Then, using the property of differentiating the original and differentiating the image, we write:

$$x'(t) \leftrightarrow pX(p) - x(0),$$

$$x''(t) \leftrightarrow p^2 X(p) - px(0) - x'(0),$$

$$tx(t) \leftrightarrow -\frac{dX(p)}{dp},$$

$$tx'(t) \leftrightarrow -\frac{d}{dp}\{pX(p) - x(0)\} = -p\frac{dX}{dp} - X(p),$$

$$tx''(t) \leftrightarrow -\frac{d}{dp}\{p^2 X(p) - px(0) - x'(0)\} = -p^2 \frac{dX}{dp} - 2pX(p) + x(0).$$

Applying the Laplace transform to a given equation, we obtain the following operator equation:

$$-p^2 \frac{dX}{dp} - 2pX(p) + x(0) - \\ -pX(p) + x(0) + p \frac{dX(p)}{dp} + X(p) + 2X(p) + 2 \frac{dX(p)}{dp} = 0 ,$$

which can be easily reduced to the form

$$(p^2 - p - 2) \frac{dX}{dp} + 3(p - 1)X(p) = 2x(0) .$$

Having solved the obtained ordinary differential equation, for example, by the method of variation of parameters, we construct its general solution:

$$X(p) = \frac{x(0)}{p-2} + \frac{c}{(p-2)(p+1)^2} .$$

Here  $C$  is an arbitrary constant. Further, since

$$\frac{1}{p-2} \leftrightarrow e^{2t} , \\ \frac{1}{(p+1)^2} \leftrightarrow te^{-t} , \\ \frac{1}{(p-2)(p+1)^2} \leftrightarrow \int_0^t \tau e^{-\tau} e^{2(t-\tau)} d\tau = \frac{1}{9} (e^{2t} - (3t+1)e^{-t}) ,$$

then the general solution of the given equation will have the form

$$x(t) = x(0)e^{2t} + c \left( \frac{1}{9} e^{2t} - \frac{1}{9} (3t+1)e^{-t} \right) = (x(0) + c)e^{2t} - c(3t+1)e^{-t} .$$

#### 1.4. APPLICATION OF THE LAPLACE TRANSFORM TO THE SOLUTION OF DIFFERENTIAL EQUATIONS WITH A DELAYED ARGUMENT

Consider a linear differential equation with a delayed argument with constant coefficients:

$$x^{(n)}(t) = \sum_{k=0}^{n-1} a_k x^{(k)}(t - \tau_k) + f(t), \quad 0 < t < +\infty, \quad (1.13)$$

where  $a_k = \text{const}$ ,  $\tau_k = \text{const} \geq 0$ .

Let's assume that

$$x(t) = x'(t) = \dots = x^{(n-1)}(t) \equiv 0,$$

for  $\forall t < 0$ .

Let it be required to find a solution to equation (1.13) satisfying the initial conditions:

$$x(0) = x'(0) = \dots = x^{(n-1)}(0) = 0. \quad (1.14)$$

Applying the Laplace transform to both parts of equation (1.13) and taking into account the delay property of the original, we obtain the operator equation for the image  $X(p) \leftrightarrow x(t)$ :

$$p^n X(p) = \sum_{k=0}^{n-1} a_k p^k X(p) e^{-\tau_k p} + F(p), \quad (1.15)$$

where  $F(p) \leftrightarrow f(t)$ .

From (1.15) for  $X(p)$  we will have



$$X(p) = \frac{F(p)}{p^n - \sum_{k=0}^{n-1} a_k p^k e^{-\tau_k p}}. \quad (1.16)$$

The original for the image (1.16) defines the solution of equation (1.13) satisfying the conditions (1.14).

Let's formulate a problem for an equation with a delayed argument describing a *process with an aftereffect*. It is required to find a continuously differentiable solution  $x(t)$  for  $t > t_0$  of the equation

$$x'(t) = f(t, x(t), x(t - \tau)), \quad \tau = \text{const} > 0, \quad (1.17)$$

if it is known that

$$x(t) = \varphi(t), \quad t \in [t_0 - \tau, t_0]. \quad (1.18)$$

The initial function  $\varphi(t)$  is a given continuously differentiable function.

The segment  $[t_0 - \tau, t_0]$  on which the function  $\varphi(t)$  is defined is called the *initial set*.

If equation (1.17) is linear, then its solution satisfying condition (1.18) can be found using the Laplace transform. Let  $t_0 = 0$ , then when constructing the corresponding operator equation, it should be taken into account that for the image of the function  $x(t - \tau)$  we have

$$\begin{aligned} x(t - \tau) &\leftrightarrow \int_0^\infty e^{-pt} x(t - \tau) dt = \int_{-\tau}^\infty e^{-p(\eta + \tau)} x(\eta) d\eta = \\ &= \int_{-\tau}^0 e^{-p(\eta + \tau)} x(\eta) d\eta + \int_0^\infty e^{-p(\eta + \tau)} x(\eta) d\eta = e^{-p\tau} \int_{-\tau}^0 e^{-p\eta} \varphi(\eta) d\eta + e^{-p\tau} X(p). \end{aligned}$$

When restoring originals from known images, you can use the following decomposition:

$$\frac{1}{1 - \frac{\gamma e^{-np}}{(p+a)^m}} = 1 + \frac{\gamma e^{-np}}{(p+a)^m} + \left( \frac{\gamma e^{-np}}{(p+a)^m} \right)^2 + \dots = \sum_{k=0}^{\infty} \left( \frac{\gamma e^{-np}}{(p+a)^m} \right)^k, \quad (1.19)$$

which is true for any  $n, m \in N$ , on condition  $\operatorname{Re} p > 0$ .

### Example 1

Find a solution of the equation

$$x'(t) = x(t-1) + 1, \quad x(0) = 0.$$

Solution:

Assuming that  $x(t) \equiv 0$  for  $t \in [-1, 0]$ , applying the Laplace transform to a given equation, we obtain the following operator equation:

$$pX(p) = X(p)e^{-p} + \frac{1}{p}.$$

Where from

$$X(p) = \frac{1}{p} \frac{1}{pe^{-p}} = \frac{1}{p^2} \frac{1}{1 - \frac{e^{-p}}{p}}.$$

Further, applying the formula (1.19), we have

$$X(p) = \frac{1}{p^2} \sum_{k=0}^{\infty} \left( \frac{e^{-p}}{p} \right)^k = \sum_{k=0}^{\infty} \frac{e^{-pk}}{p^{k+2}}.$$

Given the delay property, we construct an expression for the corresponding original  $x(t)$  in the form

$$x(t) = \sum_{k=0}^{\infty} \frac{(t-k)^{k+1}}{(k+1)!} \theta(t-k).$$

## Example 2

Find a solution of the equation

$$x'(t) = x(t-1),$$

if  $x(t) \equiv 2$  for  $\forall t \in [-1, 0]$ .

Solution:

Let  $x(t) \leftrightarrow X(p)$ .

It follows from the condition that  $x(0) = 2$ , so we have

$$x'(t) \leftrightarrow pX(p) - x(0) = pX(p) - 2.$$

We apply the Laplace transform to both parts of the given equation. For the right side of the equation, we have

$$\begin{aligned} x(t-1) &\leftrightarrow \int_0^{\infty} e^{-pt} x(t-1) dt = \int_{-1}^{\infty} e^{-p(z+1)} x(z) dz = \\ &= \int_{-1}^0 e^{-p(z+1)} x(z) dz + \int_0^{\infty} e^{-p(z+1)} x(z) dz = \\ &= 2 \int_{-1}^0 e^{-p(z+1)} dz + e^{-p} X(p) = \frac{2}{p} (1 - e^{-p}) + e^{-p} X(p). \end{aligned}$$

Therefore, the corresponding operator equation has the form

$$pX(p) - 2 = \frac{2}{p}(1 - e^{-p}) + e^{-p}X(p).$$

From here we get

$$X(p) = 2 \frac{p+1-e^{-p}}{p^2 - pe^{-p}} = \frac{2}{p} + \frac{2}{p(p-e^{-p})}.$$

Using the result of the previous example, we will construct the original in the form

$$x(t) = 2 \left( \theta(t) + \sum_{k=0}^{\infty} \frac{(t-k)^{k+1}}{(k+1)!} \theta(t-k) \right).$$

### Example 3

Find a solution of the equation

$$x'(t) + 2x(t) - x(t-1) = f(t),$$

if  $x(0) = 0$  and  $x(t) \equiv 0$  for  $\forall t < 0$ .

Solution:

Let  $x(t) \leftrightarrow X(p)$ ,  $f(t) \leftrightarrow F(p)$ .

Since under the given conditions  $x(t-1) \leftrightarrow e^{-p}X(p)$ , the operator equation corresponding to the given one has the form

$$pX(p) + 2X(p) - e^{-p}X(p) = F(p).$$

The solution of this equation is written as a product:

$$X(p) = \frac{1}{p+2-e^{-p}} F(p).$$

Let's build the original for the function

$$Y(p) = \frac{1}{p+2-e^{-p}},$$

by performing the following transformations:

$$Y(p) = \frac{1}{p+2-e^{-p}} = \frac{1}{p+2} \left( \frac{1}{1-\frac{e^{-p}}{p+2}} \right) = \sum_{k=0}^{\infty} \frac{e^{kp}}{(p+2)^{k+1}}.$$

The last equality is written, taking into account the formula (1.19).

Turning to the originals for the summands of the sum of the series, using

$t^k \leftrightarrow \frac{k!}{p^{k+1}}, t < 0$  and the delay property, we find

$$Y(p) \leftrightarrow y(t) = \sum_{k=0}^{\infty} \frac{(t-k)^k}{k!} e^{-2(t-k)} \theta(t-k).$$

The solution to this problem will be the function  $x(t)$ , which is a convolution of the functions  $f(t)$  and  $y(t)$ :

$$x(t) = \sum_{k=0}^{\infty} \frac{1}{k!} \int_0^t f(t-\tau) (\tau-k)^k e^{-2(\tau-k)} \theta(\tau-k) d\tau.$$